some progress for type soundness

Hs/HsJudgment.lean
@@ -23,23 +23,22 @@ inductive HsJudgment : (i : JIdx) -> HsCtx HsTerm -> JudgmentType i -> Prop wher
   HsJudgment .CtxJ (.empty :: Γ) ()
 | wfkind :
   HsJudgment .CtxJ Γ  () ->
-  HsJudgment .TermJ Γ (k, `□) ->
+  HsJudgment .KindJ Γ (k, `□) ->
   HsJudgment .CtxJ (.kind k ::  Γ) ()
 | wftype :
   HsJudgment .CtxJ Γ () ->
-  HsJudgment .TermJ Γ (A, `★) ->
+  HsJudgment .TypeJ Γ (A, `★) ->
   HsJudgment .CtxJ (.type A :: Γ) ()
 | wfdatatypeDecl :
   HsJudgment .CtxJ Γ () ->
-  HsJudgment .TermJ Γ (k, `□) ->
-  ∀ p: i < ctors.length, HsJudgment .TermJ (pad_empty_ctx (i - 1) ++ Γ) (ctors[i]'(by assumption), `★) ->
+  HsJudgment .KindJ Γ (T, `□) ->
+  ∀ p: i < ctors.length, HsJudgment .TypeJ (pad_empty_ctx (i - 1) ++ .type T :: Γ) (ctors[i]'(by assumption), `★) ->
   HsJudgment .CtxJ (.datatypeDecl k ctors :: Γ) ()
 | wfterm :
   HsJudgment .CtxJ Γ () ->
-  HsJudgment .TermJ Γ (A, `★) ->
+  HsJudgment .TypeJ Γ (A, `★) ->
   HsJudgment .TermJ Γ (t, A) ->
   HsJudgment .CtxJ (.term A t :: Γ) ()
-
 
 | wfstar :
   HsJudgment .CtxJ Γ () ->
@@ -50,24 +49,55 @@ inductive HsJudgment : (i : JIdx) -> HsCtx HsTerm -> JudgmentType i -> Prop wher
   HsJudgment .KindJ Γ (κ2, `□) ->
   HsJudgment .KindJ Γ (κ1 `-k> κ2, `□)
 
-
 | varTy :
   HsJudgment .CtxJ Γ () ->
-  (Γ s@ x) = .type T ∨ (Γ s@ x) = .tycon T ->
-  HsJudgment .TypeJ Γ (`#x, T)
+  (Γ s@ x) = .tycon T ∨ (Γ s@ x) = .kind T ->
+  HsJudgment .TermJ Γ (`#x, T)
 
-| arrowt :
+| arrow :
   HsJudgment .CtxJ Γ () ->
   HsJudgment .TypeJ Γ (A, `★) ->
   HsJudgment .TypeJ (.empty :: Γ) (B, `★) ->
   HsJudgment .TypeJ Γ (A → B, `★)
-| allt :
+| all :
   HsJudgment .CtxJ Γ () ->
   HsJudgment .KindJ Γ (A, `□) ->
   HsJudgment .TypeJ (.kind A :: Γ) (B, `★) ->
   HsJudgment .TypeJ Γ (`∀{A} B, `★)
-| appt :
+| appk :
   HsJudgment .CtxJ Γ () ->
   HsJudgment .TypeJ Γ (T, k `-k> k') ->
   HsJudgment .TypeJ Γ (A, k) ->
   HsJudgment .TypeJ Γ (T `•k A, k')
+
+
+notation:170 Γ:170 " ⊢s " t:170 " : " A:170 => HsJudgment JIdx.TermJ Γ (t, A)
+notation:170 "⊢s " Γ:170 => HsJudgment JIdx.CtxJ Γ ()
+
+theorem hs_judgment_ctx_wf : HsJudgment v Γ idx -> HsJudgment .CtxJ Γ () := by
+intro j
+induction j
+all_goals try simp [*]
+case _ => constructor
+case _ ih => constructor; apply ih
+case _ j _ _ ih => constructor; apply j; assumption
+case _ j _ _ ih => constructor; apply j; assumption
+case _ j _ _ ih => constructor; assumption; assumption; assumption
+case _ j _ h _ ih => constructor; assumption; assumption; assumption
+
+inductive HsFrameWf : HsCtx HsTerm -> HsFrame HsTerm -> Prop
+| empty :
+  ⊢s Γ ->
+  HsFrameWf Γ .empty
+| kind:
+  Γ ⊢s K : `★ ->
+  HsFrameWf Γ (.kind K)
+| type:
+  Γ ⊢s A : `★ ->
+  HsFrameWf Γ (.type A)
+| datatypeDecl:
+  Γ ⊢s T : `★ ->
+  ∀ p: i < ctors.length, HsJudgment .TermJ (pad_empty_ctx (i - 1) ++ Γ) (ctors[i]'(by assumption), `★) ->
+  HsFrameWf Γ (.datatypeDecl T ctors)
+
+notation:170 Γ:170 " ⊢s " f:170 => HsFrameWf Γ f
